cpo.v
@@ -20,27 +20,41 @@ From algco Require Import
 
 Local Open Scope order_scope.
 
-(** [A] is a CPO (complete partial order) whenever suprema of countable
-    collections exist. *)
-Class CPO (A : Type) `{OType A} : Prop :=
-  { exists_sup : forall f : nat -> A, exists s, supremum s f }.
-
 (** [A] is a dCPO (directed-complete partial order) whenever suprema of
     directed countable collections exist. *)
 Class dCPO (A : Type) `{OType A} : Prop :=
-  { exists_dsup : forall f : nat -> A, directed f -> exists s, supremum s f }.
-
-(** [A] is a lCPO (lower-complete partial order) whenever infima of
-    countable collections exist. *)
-Class lCPO (A : Type) `{OType A} : Prop :=
-  { exists_inf : forall f : nat -> A, exists s, infimum s f }.
+  { exists_sup : forall f : nat -> A, directed f -> exists s, supremum s f }.
 
 (** [A] is a ldCPO (lower-directed-complete partial order) whenever
     infima of downward-directed countable collections exist. *)
 Class ldCPO (A : Type) `{OType A} : Prop :=
-  { exists_dinf : forall f : nat -> A, downward_directed f -> exists s, infimum s f }.
+  { exists_inf : forall f : nat -> A, downward_directed f -> exists s, infimum s f }.
 
-Class Lattice (A : Type) {o : OType A} `{@CPO A o} `{@lCPO A o} : Prop := {}.
+Class dLattice (A : Type) {o : OType A} `{@dCPO A o} `{@ldCPO A o} : Prop := {}.
+
+(** Pointed lattice.  For convenience -- deviates slightly from
+    standard definition by quantifying over only countable
+    collections. *)
+Class pLattice (A : Type) {o : OType A} {p : @PType _ o} : Prop := {
+    lattice_exists_sup : forall f : nat -> A, exists s, supremum s f
+  ; lattice_exists_inf : forall f : nat -> A, exists s, infimum s f
+  }.
+
+#[global]
+  Instance pLattice_dCPO {A} `{pLattice A} : dCPO A.
+Proof. firstorder. Qed.
+#[global] Hint Resolve pLattice_dCPO : order.
+
+#[global]
+  Instance pLattice_ldCPO {A} `{pLattice A} : ldCPO A.
+Proof. firstorder. Qed.
+#[global] Hint Resolve pLattice_ldCPO : order.
+
+#[global]
+  Instance pLattice_dLattice {A} `{pLattice A} : dLattice A.
+Qed.
+#[global] Hint Resolve pLattice_dLattice : order.
+
 
 Lemma ex_ex_supremum {A} `{OType A} (f : nat -> A) :
   exists x : A, (exists b : A, supremum b f) -> supremum x f.
@@ -75,126 +89,143 @@ Definition inf_prim {A} `{OType A} (f : nat -> A)
 (* Take the supremum of countable collection [f]. *)
 Definition sup {A} `{OType A} (f : nat -> A) : A := proj1_sig (sup_prim f).
 
-(* [sup f] is the supremum of [f] whenever [A] is a CPO. *)
-Lemma sup_spec {A} `{CPO A} (f : nat -> A) : supremum (sup f) f.
-Proof. unfold sup; destruct (sup_prim f) as [a Ha]; apply Ha, H0. Qed.
-
 (* [sup f] is the supremum of [f] whenever [A] is a dCPO and [f] is
    directed. *)
-Lemma dsup_spec {A} `{dCPO A} (f : nat -> A) :
+Lemma sup_spec {A} `{dCPO A} (f : nat -> A) :
   directed f -> supremum (sup f) f.
 Proof. intro Hf; unfold sup; destruct sup_prim; simpl; apply s, H0; auto. Qed.
+
+Lemma lattice_sup_spec {A} `{pLattice A} (f : nat -> A) :
+  supremum (sup f) f.
+Proof. unfold sup; destruct sup_prim; simpl; apply s; firstorder. Qed.
 
 (* Take the infimum of countable collection [f]. *)
 Definition inf {A} `{OType A} (f : nat -> A) : A := proj1_sig (inf_prim f).
 
-(* [inf f] is the infimum of [f] whenever [A] is an lCPO. *)
-Lemma inf_spec {A} `{lCPO A} (f : nat -> A) : infimum (inf f) f.
-Proof. unfold inf; destruct (inf_prim f) as [a Ha]; apply Ha, H0. Qed.
-
 (* [inf f] is the infimum of [f] whenever [A] is an ldCPO and [f] is
    downward-directed. *)
-Lemma dinf_spec {A} `{ldCPO A} (f : nat -> A) :
+Lemma inf_spec {A} `{ldCPO A} (f : nat -> A) :
   downward_directed f -> infimum (inf f) f.
 Proof. intro Hf; unfold inf; destruct inf_prim; simpl; apply i, H0; auto. Qed.
 
-#[global]
-  Instance CPO_dCPO {A} `{CPO A} : dCPO A.
-Proof. constructor; intros f Hf; apply H0. Qed.
-#[global] Hint Resolve CPO_dCPO : order.
+Lemma lattice_inf_spec {A} `{pLattice A} (f : nat -> A) :
+  infimum (inf f) f.
+Proof. unfold inf; destruct inf_prim; simpl; apply i; firstorder. Qed.
 
 #[global]
-  Instance lCPO_ldCPO {A} `{lCPO A} : ldCPO A.
-Proof. constructor; intros f Hf; apply H0. Qed.
-#[global] Hint Resolve lCPO_ldCPO : order.
+  Instance pLattice_arrow {A B} `{pLattice B} : pLattice (A -> B).
+Proof.
+  constructor; intro f.
+  - exists (fun x => sup (fun i => f i x)).
+    apply supremum_apply.
+    intro a; apply lattice_sup_spec.
+  - exists (fun x => inf (fun i => f i x)).
+    apply infimum_apply.
+    intro a; apply lattice_inf_spec.
+Qed.
+#[global] Hint Resolve pLattice_arrow : order.
 
 (** [Prop] has suprema and infima. *)
 
-#[global]
-  Instance CPO_Prop : CPO Prop.
-Proof.
-  constructor; intro f; exists (exists i, f i); split.
-  - intros i Hi; exists i; auto.
-  - intros ub Hub [i Hi]; eapply Hub; eauto.
-Qed.
-#[global] Hint Resolve CPO_Prop : order.
+(* #[global] *)
+(*   Instance dCPO_Prop : dCPO Prop. *)
+(* Proof. *)
+(*   constructor; intro f; exists (exists i, f i); split. *)
+(*   - intros i Hi; exists i; auto. *)
+(*   - intros ub Hub [i Hi]; eapply Hub; eauto. *)
+(* Qed. *)
+(* #[global] Hint Resolve dCPO_Prop : order. *)
+
+(* #[global] *)
+(*   Instance ldCPO_Prop : ldCPO Prop. *)
+(* Proof. *)
+(*   constructor; intros f; exists (forall i, f i); split. *)
+(*   - intros i Hi; auto. *)
+(*   - intros ub Hub x i; apply Hub; auto. *)
+(* Qed. *)
+(* #[global] Hint Resolve ldCPO_Prop : order. *)
+
+(* #[global] *)
+(*   Instance dLattice_Prop : dLattice Prop. Qed. *)
+(* #[global] Hint Resolve dLattice_Prop : order. *)
 
 #[global]
-  Instance lCPO_Prop : lCPO Prop.
+  Instance Lattice_Prop : pLattice Prop.
 Proof.
-  constructor; intros f; exists (forall i, f i); split.
-  - intros i Hi; auto.
-  - intros ub Hub x i; apply Hub; auto.
+  constructor; intro f.
+  - exists (exists i, f i); split.
+    + intros i Hi; exists i; auto.
+    + intros ub Hub [i Hi]; eapply Hub; eauto.
+  - exists (forall i, f i); split.
+    + intros i Hi; auto.
+    + intros ub Hub x i; apply Hub; auto.
 Qed.
-#[global] Hint Resolve lCPO_Prop : order.
-
-#[global]
-  Instance Lattice_Prop : Lattice Prop. Qed.
 #[global] Hint Resolve Lattice_Prop : order.
 
+(* #[global] *)
+(*   Instance dCPO_bool : dCPO bool. *)
+(* Proof. *)
+(*   constructor; intro f. *)
+(*   destruct (classic (exists i, f i = true)). *)
+(*   - exists true; split. *)
+(*     + intro i; simpl; unfold bool_le; destruct (f i); auto. *)
+(*     + intros x Hx; destruct x; try reflexivity. *)
+(*       destruct H as [i H]; specialize (Hx i). *)
+(*       rewrite H in Hx; destruct Hx. *)
+(*   - exists false; split. *)
+(*     + intro i; destruct (f i) eqn:Hfi; try reflexivity. *)
+(*       exfalso; apply H; exists i; auto. *)
+(*     + intros x Hx; destruct x; reflexivity. *)
+(* Qed. *)
+(* #[global] Hint Resolve dCPO_bool : order. *)
+
+(* #[global] *)
+(*   Instance ldCPO_bool : ldCPO bool. *)
+(* Proof. *)
+(*   constructor; intro f. *)
+(*   destruct (classic (exists i, f i = false)). *)
+(*   - exists false; split. *)
+(*     + intro i; simpl; unfold bool_le; destruct (f i); auto. *)
+(*     + intros x Hx; destruct x; try reflexivity. *)
+(*       destruct H as [i H]; specialize (Hx i). *)
+(*       rewrite H in Hx; destruct Hx. *)
+(*   - exists true; split. *)
+(*     + intro i; destruct (f i) eqn:Hfi; try reflexivity. *)
+(*       exfalso; apply H; exists i; auto. *)
+(*     + intros x Hx; destruct x; reflexivity. *)
+(* Qed. *)
+(* #[global] Hint Resolve ldCPO_bool : order. *)
+
+(* #[global] *)
+(*   Instance dLattice_bool : dLattice bool. Qed. *)
+(* #[global] Hint Resolve dLattice_bool : order. *)
+
 #[global]
-  Instance CPO_bool : CPO bool.
+  Instance Lattice_bool : pLattice bool.
 Proof.
   constructor; intro f.
-  destruct (classic (exists i, f i = true)).
-  - exists true; split.
-    + intro i; simpl; unfold bool_le; destruct (f i); auto.
-    + intros x Hx; destruct x; try reflexivity.
-      destruct H as [i H]; specialize (Hx i).
-      rewrite H in Hx; destruct Hx.
-  - exists false; split.
-    + intro i; destruct (f i) eqn:Hfi; try reflexivity.
-      exfalso; apply H; exists i; auto.
-    + intros x Hx; destruct x; reflexivity.
+  - destruct (classic (exists i, f i = true)).
+    + exists true; split.
+      * intro i; simpl; unfold bool_le; destruct (f i); auto.
+      * intros x Hx; destruct x; try reflexivity.
+        destruct H as [i H]; specialize (Hx i).
+        rewrite H in Hx; destruct Hx.
+    + exists false; split.
+      * intro i; destruct (f i) eqn:Hfi; try reflexivity.
+        exfalso; apply H; exists i; auto.
+      * intros x Hx; destruct x; reflexivity.
+  - destruct (classic (exists i, f i = false)).
+    + exists false; split.
+      * intro i; simpl; unfold bool_le; destruct (f i); auto.
+      * intros x Hx; destruct x; try reflexivity.
+        destruct H as [i H]; specialize (Hx i).
+        rewrite H in Hx; destruct Hx.
+    + exists true; split.
+      * intro i; destruct (f i) eqn:Hfi; try reflexivity.
+        exfalso; apply H; exists i; auto.
+      * intros x Hx; destruct x; reflexivity.
 Qed.
-#[global] Hint Resolve CPO_bool : order.
-
-#[global]
-  Instance lCPO_bool : lCPO bool.
-Proof.
-  constructor; intro f.
-  destruct (classic (exists i, f i = false)).
-  - exists false; split.
-    + intro i; simpl; unfold bool_le; destruct (f i); auto.
-    + intros x Hx; destruct x; try reflexivity.
-      destruct H as [i H]; specialize (Hx i).
-      rewrite H in Hx; destruct Hx.
-  - exists true; split.
-    + intro i; destruct (f i) eqn:Hfi; try reflexivity.
-      exfalso; apply H; exists i; auto.
-    + intros x Hx; destruct x; reflexivity.
-Qed.
-#[global] Hint Resolve lCPO_bool : order.
-
-#[global]
-  Instance Lattice_bool : Lattice bool. Qed.
-#[global] Hint Resolve Lattice_bool : order.
-
-Lemma ge_inf {A} `{lCPO A} (f : nat -> A) (a : A) (i : nat) :
-  f i ⊑ a ->
-  inf f ⊑ a.
-Proof.
-  intros Hleq; generalize (inf_spec f); intros [Hub Hlub]; auto.
-  etransitivity; eauto.
-Qed.
-
-Lemma le_inf {A} `{lCPO A} (f : nat -> A) (a : A) :
-  lower_bound a f ->
-  a ⊑ inf f.
-Proof. intros Hbound; generalize (inf_spec f); intros [Hlb Hglb]; auto. Qed.
-
-Lemma ge_sup {A} `{CPO A} (f : nat -> A) (a : A) :
-  upper_bound a f ->
-  sup f ⊑ a.
-Proof. intros Hbound; generalize (sup_spec f); intros [Hub Hlub]; auto. Qed.
-
-Lemma le_sup {A} `{CPO A} (f : nat -> A) (a : A) (i : nat) :
-  a ⊑ f i ->
-  a ⊑ sup f.
-Proof.
-  intros Hleq; generalize (sup_spec f); intros [Hub Hlub]; auto.
-  etransitivity; eauto.
-Qed.
+#[global] Hint Resolve Lattice_Prop : order.
 
 #[global]
   Instance ldCPO_arrow {A B} `{ldCPO B} : ldCPO (A -> B).
@@ -207,21 +238,11 @@ Proof.
     exists l; auto. }
   split.
   - intros i x; specialize (Hf' x).
-    apply dinf_spec in Hf'; apply Hf'.
+    apply inf_spec in Hf'; apply Hf'.
   - intros g Hlb x.
     specialize (Hf' x).
-    apply dinf_spec in Hf'.
+    apply inf_spec in Hf'.
     apply Hf'; intro; apply Hlb.
-Qed.
-
-#[global]
-  Instance lCPO_arrow {A B} `{lCPO B} : lCPO (A -> B).
-Proof.
-  constructor; intros f.
-  exists (fun x => inf (fun n => f n x)).
-  split.
-  - intros i x; eapply ge_inf; reflexivity.
-  - intros g Hg x; apply le_inf; intro i; apply Hg.
 Qed.
 
 #[global]
@@ -235,21 +256,11 @@ Proof.
     exists l; auto. }
   split.
   - intros i x; specialize (Hf' x).
-    apply dsup_spec in Hf'; apply Hf'.
+    apply sup_spec in Hf'; apply Hf'.
   - intros g Hub x.
     specialize (Hf' x).
-    apply dsup_spec in Hf'.
+    apply sup_spec in Hf'.
     apply Hf'; intro; apply Hub.
-Qed.
-
-#[global]
-  Instance CPO_arrow {A B} `{CPO B} : CPO (A -> B).
-Proof.
-  constructor; intros f.
-  exists (fun x => sup (fun n => f n x)).
-  split.
-  - intros i x; eapply le_sup; reflexivity.
-  - intros g Hg x; apply ge_sup; intro i; apply Hg.
 Qed.
 
 #[global]
@@ -257,11 +268,11 @@ Qed.
 Proof.
   constructor; intros ch Hch.
   destruct H0.
-  specialize (exists_dsup0 (fst ∘ ch) (directed_fst _ Hch)).
-  destruct exists_dsup0 as [a Ha].
+  specialize (exists_sup0 (fst ∘ ch) (directed_fst _ Hch)).
+  destruct exists_sup0 as [a Ha].
   destruct H2.
-  specialize (exists_dsup0 (snd ∘ ch) (directed_snd _ Hch)).
-  destruct exists_dsup0 as [b Hb].
+  specialize (exists_sup0 (snd ∘ ch) (directed_snd _ Hch)).
+  destruct exists_sup0 as [b Hb].
   exists (a, b); apply supremum_prod; auto.
 Qed.
 
@@ -285,7 +296,7 @@ Proof.
       - destruct (ch k) eqn:Hchk.
         + destruct (ch z) eqn:Hchz; auto; inv Hjz.
         + destruct (ch z) eqn:Hchz; try reflexivity; inv Hjz. }
-    destruct H0; apply exists_dsup0 in Hch_a; clear exists_dsup0.
+    destruct H0; apply exists_sup0 in Hch_a; clear exists_sup0.
     destruct (classic (exists i b, ch i = inr b)).
     { destruct H0 as [j [b Hb]].
       specialize (Hch i j).
@@ -324,7 +335,7 @@ Proof.
     - destruct (ch k) eqn:Hchk.
       + destruct (ch z) eqn:Hchz; try reflexivity; inv Hjz.
       + destruct (ch z) eqn:Hchz; auto; inv Hjz. }
-  destruct H2; apply exists_dsup0 in Hch_b; clear exists_dsup0.
+  destruct H2; apply exists_sup0 in Hch_b; clear exists_sup0.
   destruct Hch_b as [y [Hub Hlub]].
   exists (inr y); split.
   - intro i; specialize (Hub i).
@@ -345,79 +356,71 @@ Proof.
       destruct (ch i); auto; inv Hx.
 Qed.
 
-Lemma sup_const {A} `{CPO A} (a : A) :
-  sup (fun _ => a) === a.
-Proof.
-  eapply supremum_unique.
-  { apply sup_spec; auto with order. }
-  apply supremum_const.
-Qed.
-
-Lemma sup_const' {A} `{CPO A} (f : nat -> A) (a : A) :
-  f === const a ->
-  sup f === a.
-Proof.
-  intro Hf.
-  rewrite equ_arrow in Hf.
-  unfold const in Hf.
-  eapply supremum_unique.
-  - apply sup_spec; intros ? j; exists j; split; rewrite !Hf; reflexivity.
-  - apply supremum_const'; apply equ_arrow; intro i; apply Hf.
-Qed.
-
-Lemma inf_const {A} `{lCPO A} (a : A) :
-  inf (fun _ => a) === a.
-Proof.
-  eapply infimum_unique.
-  { apply inf_spec; auto with order. }
-  apply infimum_const.
-Qed.
-
-Lemma inf_const' {A} `{lCPO A} (f : nat -> A) (a : A) :
-  f === const a ->
-  inf f === a.
-Proof.
-  intro Hf.
-  rewrite equ_arrow in Hf.
-  unfold const in Hf.
-  eapply infimum_unique.
-  - apply inf_spec; intros ? j; exists j; split; rewrite !Hf; reflexivity.
-  - apply infimum_const'; apply equ_arrow; intro i; apply Hf.
-Qed.
-
-Lemma le_dsup {A} `{dCPO A} (f : nat -> A) (a : A) (i : nat) :
+Lemma le_sup {A} `{dCPO A} (f : nat -> A) (a : A) (i : nat) :
   directed f ->
   a ⊑ f i ->
   a ⊑ sup f.
 Proof.
   intros Hf Hleq.
-  generalize (dsup_spec f); intros [Hub Hlub]; auto.
+  generalize (sup_spec f); intros [Hub Hlub]; auto.
   etransitivity; eauto.
 Qed.
 
-Lemma le_dinf {A} `{ldCPO A} (f : nat -> A) (a : A) :
+Lemma lattice_le_sup {A} `{pLattice A} (f : nat -> A) (a : A) (i : nat) :
+  a ⊑ f i ->
+  a ⊑ sup f.
+Proof.
+  intros Hleq.
+  generalize (lattice_sup_spec f); intros [Hub Hlub]; auto.
+  etransitivity; eauto.
+Qed.
+
+Lemma le_inf {A} `{ldCPO A} (f : nat -> A) (a : A) :
   downward_directed f ->
   lower_bound a f ->
   a ⊑ inf f.
 Proof.
-  intros Hf Hbound; generalize (dinf_spec f); intros [Hlb Hglb]; auto.
+  intros Hf Hbound; generalize (inf_spec f); intros [Hlb Hglb]; auto.
 Qed.
 
-Lemma ge_dsup {A} `{dCPO A} (f : nat -> A) (a : A) :
+Lemma lattice_le_inf {A} `{pLattice A} (f : nat -> A) (a : A) :
+  lower_bound a f ->
+  a ⊑ inf f.
+Proof.
+  intros Hbound; generalize (lattice_inf_spec f); intros [Hlb Hglb]; auto.
+Qed.
+
+Lemma ge_sup {A} `{dCPO A} (f : nat -> A) (a : A) :
   directed f ->
   upper_bound a f ->
   sup f ⊑ a.
 Proof.
-  intros Hf Hbound; generalize (dsup_spec f); intros [Hub Hlub]; auto.
+  intros Hf Hbound; generalize (sup_spec f); intros [Hub Hlub]; auto.
 Qed.
 
-Lemma ge_dinf {A} `{ldCPO A} (f : nat -> A) (a : A) (i : nat) :
+Lemma lattice_ge_sup {A} `{pLattice A} (f : nat -> A) (a : A) :
+  upper_bound a f ->
+  sup f ⊑ a.
+Proof.
+  intros Hbound; generalize (lattice_sup_spec f); intros [Hub Hlub]; auto.
+Qed.
+
+Lemma ge_inf {A} `{ldCPO A} (f : nat -> A) (a : A) (i : nat) :
   downward_directed f ->
   f i ⊑ a ->
   inf f ⊑ a.
 Proof.
   intros Hf Hleq.
-  generalize (dinf_spec f); intros [Hub Hlub]; auto.
+  generalize (inf_spec f); intros [Hub Hlub]; auto.
+  etransitivity; eauto.
+Qed.
+
+Lemma lattice_ge_inf {A} `{pLattice A} (f : nat -> A) (a : A) (i : nat) :
+  f i ⊑ a ->
+  inf f ⊑ a.
+Proof.
+  intros Hleq.
+  generalize (lattice_inf_spec f); intros [Hub Hlub]; auto.
   etransitivity; eauto.
 Qed.
 
@@ -437,26 +440,32 @@ Proof.
   unfold inf; destruct (inf_prim f); apply i; exists a; auto.
 Qed.
 
-Lemma sup_apply {A B} `{CPO B} (f : nat -> A -> B) (x : A) :
-  sup f x === sup (fun i => f i x).
-Proof.
-  symmetry.
-  apply supremum_sup; auto with order.
-  apply apply_supremum, sup_spec; auto.
-Qed.
-
-Lemma dsup_apply {A B} `{dCPO B} (f : nat -> A -> B) (x : A) :
+Lemma sup_apply {A B} `{dCPO B} (f : nat -> A -> B) (x : A) :
   directed f ->
   sup f x === sup (fun i => f i x).
 Proof.
-  intro Hf; symmetry; apply supremum_sup, apply_supremum, dsup_spec; auto.
+  intro Hf; symmetry; apply supremum_sup, apply_supremum, sup_spec; auto.
 Qed.
 
-Lemma inf_apply {A B} `{lCPO B} (f : nat -> A -> B) (x : A) :
+Lemma lattice_sup_apply {A B} `{pLattice B} (f : nat -> A -> B) (x : A) :
+  sup f x === sup (fun i => f i x).
+Proof.
+  symmetry; apply supremum_sup, apply_supremum, lattice_sup_spec; auto.
+Qed.
+
+Lemma inf_apply {A B} `{ldCPO B} (f : nat -> A -> B) (x : A) :
+  downward_directed f ->
   inf f x === inf (fun i => f i x).
 Proof.
   symmetry; apply infimum_inf; auto with order.
   apply apply_infimum, inf_spec; auto.
+Qed.
+
+Lemma lattice_inf_apply {A B} `{pLattice B} (f : nat -> A -> B) (x : A) :
+  inf f x === inf (fun i => f i x).
+Proof.
+  symmetry; apply infimum_inf; auto with order.
+  apply apply_infimum, lattice_inf_spec; auto.
 Qed.
 
 Lemma continuous_sup {A B} `{dCPO A} `{dCPO B} (f : A -> B) (ch : nat -> A) :
@@ -466,7 +475,7 @@ Lemma continuous_sup {A B} `{dCPO A} `{dCPO B} (f : A -> B) (ch : nat -> A) :
 Proof.
   intros Hf Hch; symmetry.
   apply supremum_sup, Hf; auto.
-  apply dsup_spec; auto.
+  apply sup_spec; auto.
 Qed.
 
 Lemma cocontinuous_sup {A B} `{dCPO A} `{ldCPO B} (f : A -> B) (ch : nat -> A) :
@@ -476,7 +485,7 @@ Lemma cocontinuous_sup {A B} `{dCPO A} `{ldCPO B} (f : A -> B) (ch : nat -> A) :
 Proof.
   intros Hf Hch; symmetry.
   apply infimum_inf, Hf; auto.
-  apply dsup_spec; auto.
+  apply sup_spec; auto.
 Qed.
 
 Lemma wcontinuous_sup {A B} `{dCPO A} `{dCPO B} (f : A -> B) (ch : nat -> A) :
@@ -486,7 +495,7 @@ Lemma wcontinuous_sup {A B} `{dCPO A} `{dCPO B} (f : A -> B) (ch : nat -> A) :
 Proof.
   intros Hf Hch; symmetry.
   apply supremum_sup, Hf; auto.
-  apply dsup_spec; auto with order.
+  apply sup_spec; auto with order.
 Qed.
 
 Lemma dec_continuous_inf {A B} `{ldCPO A} `{ldCPO B} (f : A -> B) (ch : nat -> A) :
@@ -496,7 +505,7 @@ Lemma dec_continuous_inf {A B} `{ldCPO A} `{ldCPO B} (f : A -> B) (ch : nat -> A
 Proof.
   intros Hf Hch; symmetry.
   apply infimum_inf, Hf; auto.
-  apply dinf_spec; auto.
+  apply inf_spec; auto.
 Qed.
 
 Lemma dec_cocontinuous_inf {A B} `{ldCPO A} `{dCPO B} (f : A -> B) (ch : nat -> A) :
@@ -506,7 +515,7 @@ Lemma dec_cocontinuous_inf {A B} `{ldCPO A} `{dCPO B} (f : A -> B) (ch : nat -> 
 Proof.
   intros Hf Hch; symmetry.
   apply supremum_sup, Hf; auto.
-  apply dinf_spec; auto.
+  apply inf_spec; auto.
 Qed.
 
 Lemma dec_wcontinuous_inf {A B} `{ldCPO A} `{ldCPO B} (f : A -> B) (ch : nat -> A) :
@@ -516,7 +525,7 @@ Lemma dec_wcontinuous_inf {A B} `{ldCPO A} `{ldCPO B} (f : A -> B) (ch : nat -> 
 Proof.
   intros Hf Hch; symmetry.
   apply infimum_inf, Hf; auto.
-  apply dinf_spec; auto with order.
+  apply inf_spec; auto with order.
 Qed.
 
 Lemma Proper_sup {A} `{dCPO A} (f g : nat -> A) :
@@ -527,8 +536,8 @@ Lemma Proper_sup {A} `{dCPO A} (f g : nat -> A) :
 Proof.
   intros Hf Hg Hfg.
   eapply supremum_unique.
-  - apply dsup_spec; auto.
-  - rewrite Hfg; apply dsup_spec; auto.
+  - apply sup_spec; auto.
+  - rewrite Hfg; apply sup_spec; auto.
 Qed.
 
 Lemma sup_shift {A} `{dCPO A} (f : nat -> A) :
@@ -537,7 +546,7 @@ Lemma sup_shift {A} `{dCPO A} (f : nat -> A) :
 Proof.
   intro Hf; apply supremum_sup; auto with order.
   apply supremum_shift; auto.
-  apply dsup_spec; auto with order.
+  apply sup_spec; auto with order.
 Qed.
 
 Lemma sup_shift' {A} `{dCPO A} (f g : nat -> A) :
@@ -548,7 +557,7 @@ Proof.
   intros Hch Heq; subst.
   symmetry.
   apply supremum_sup.
-  rewrite Heq; apply supremum_shift, dsup_spec; auto with order.
+  rewrite Heq; apply supremum_shift, sup_spec; auto with order.
 Qed.
 
 Lemma inf_shift' {A} `{ldCPO A} (f g : nat -> A) :
@@ -559,26 +568,26 @@ Proof.
   intros Hch Heq; subst.
   symmetry.
   apply infimum_inf.
-  rewrite Heq; apply infimum_shift, dinf_spec; auto with order.
+  rewrite Heq; apply infimum_shift, inf_spec; auto with order.
 Qed.
 
-Lemma dsup_intro (P : nat -> Prop) (i : nat) :
+Lemma sup_intro (P : nat -> Prop) (i : nat) :
   directed P ->
   P i ->
   sup P.
 Proof.
   intros Hdir HP.
-  generalize (dsup_spec _ Hdir); intros [Hub Hlub].
+  generalize (sup_spec _ Hdir); intros [Hub Hlub].
   eapply Hub; eauto.
 Qed.
 
-Lemma dsup_elim (P : nat -> Prop) :
+Lemma sup_elim (P : nat -> Prop) :
   directed P ->
   sup P ->
   exists i, P i.
 Proof.
   intros Hdir HP.
-  generalize (dsup_spec _ Hdir); intros [Hub Hlub].
+  generalize (sup_spec _ Hdir); intros [Hub Hlub].
   apply Hlub; auto.
   intros i H'; exists i; apply H'.
 Qed.
@@ -613,7 +622,7 @@ Proof.
 Qed.
 
 (** [dec_iter F z] is a fixed point of [F]. *)
-Lemma dec_iter_unfold {A} `{lCPO A} (F : A -> A) (z : A) :
+Lemma dec_iter_unfold {A} `{ldCPO A} (F : A -> A) (z : A) :
   dec_wcontinuous F ->
   F z ⊑ z ->
   dec_iter F z === F (dec_iter F z).
@@ -630,46 +639,30 @@ Proof.
   apply equ_arrow; intro i; reflexivity.
 Qed.
 
-Lemma dsup_apply_ext {A B} `{dCPO B} {_ : ExtType B} (f : nat -> A -> B) (x : A) :
+Lemma sup_apply_ext {A B} `{dCPO B} {_ : ExtType B} (f : nat -> A -> B) (x : A) :
   directed f ->
   sup f x = sup (fun i => f i x).
 Proof.
-  intro Hf; symmetry; apply ext, supremum_sup, apply_supremum, dsup_spec; auto.
+  intro Hf; symmetry; apply ext, supremum_sup, apply_supremum, sup_spec; auto.
 Qed.
 
-Lemma monotone_dsup {A} `{dCPO A} (f g : nat -> A) :
+Lemma monotone_sup {A} `{dCPO A} (f g : nat -> A) :
   directed f ->
   directed g ->
   (forall i, f i ⊑ g i) ->
   sup f ⊑ sup g.
 Proof.
-  intros Hf Hg Hfg; apply ge_dsup; auto.
-  intro i; etransitivity; eauto; apply dsup_spec; auto.
-Qed.
-
-Lemma monotone_sup {A} `{CPO A} (f g : nat -> A) :
-  (forall i, f i ⊑ g i) ->
-  sup f ⊑ sup g.
-Proof.
-  intros Hfg; apply ge_sup; auto.
+  intros Hf Hg Hfg; apply ge_sup; auto.
   intro i; etransitivity; eauto; apply sup_spec; auto.
 Qed.
 
-Lemma monotone_dinf {A} `{ldCPO A} (f g : nat -> A) :
+Lemma monotone_inf {A} `{ldCPO A} (f g : nat -> A) :
   downward_directed f ->
   downward_directed g ->
   (forall i, f i ⊑ g i) ->
   inf f ⊑ inf g.
 Proof.
-  intros Hf Hg Hfg; apply le_dinf; auto.
-  intro i; etransitivity; eauto; apply dinf_spec; auto.
-Qed.
-
-Lemma monotone_inf {A} `{lCPO A} (f g : nat -> A) :
-  (forall i, f i ⊑ g i) ->
-  inf f ⊑ inf g.
-Proof.
-  intros Hfg; apply le_inf; auto.
+  intros Hf Hg Hfg; apply le_inf; auto.
   intro i; etransitivity; eauto; apply inf_spec; auto.
 Qed.
 
@@ -679,7 +672,7 @@ Lemma Proper_inf {A} `{ldCPO A} (f g : nat -> A) :
   f === g ->
   inf f === inf g.
 Proof.
-  intros Hf Hg Hfg; split; apply monotone_dinf; auto; intro i; apply Hfg.
+  intros Hf Hg Hfg; split; apply monotone_inf; auto; intro i; apply Hfg.
 Qed.
 
 Lemma continuous_supP {A} `{dCPO A} (f : A -> Prop) (ch : nat -> A) :
@@ -689,6 +682,26 @@ Lemma continuous_supP {A} `{dCPO A} (f : A -> Prop) (ch : nat -> A) :
 Proof.
   intros Hf Hch.
   apply equ_iff, continuous_sup; auto.
+Qed.
+
+Lemma sup_const {A} `{dCPO A} (a : A) :
+  sup (fun _ => a) === a.
+Proof.
+  eapply supremum_unique.
+  { apply sup_spec; auto with order. }
+  apply supremum_const.
+Qed.
+
+Lemma sup_const' {A} `{dCPO A} (f : nat -> A) (a : A) :
+  f === const a ->
+  sup f === a.
+Proof.
+  intro Hf.
+  rewrite equ_arrow in Hf.
+  unfold const in Hf.
+  eapply supremum_unique.
+  - apply sup_spec; intros ? j; exists j; split; rewrite !Hf; reflexivity.
+  - apply supremum_const'; apply equ_arrow; intro i; apply Hf.
 Qed.
 
 Lemma sup_true_exists_i (f : nat -> bool) :
